LeanStatefulAoc.lean
@@ -1,6 +1,7 @@
 import LeanStatefulAoc.Basic
 import LeanStatefulAoc.Choice
 import LeanStatefulAoc.Combinators
+import LeanStatefulAoc.CodeEval
 import LeanStatefulAoc.Computation
 import LeanStatefulAoc.Firewall
 import LeanStatefulAoc.Heyting
